{-# OPTIONS --exact-split --safe #-}

open import Data.Nat using (â„• ; zero ; suc) renaming (_+_ to _+â„•_)
open import Data.Product using (_Ã—_ ; _,_) renaming (projâ‚ to fst ; projâ‚‚ to snd)
open import Data.Sum renaming (_âŠ_ to _+_ ; injâ‚ to inl ; injâ‚‚ to inr)
open import Data.Unit renaming (âŠ¤ to ğŸ™ ; tt to âˆ—)
open import Data.Empty
open import Data.Fin using (Fin)

open import Level renaming (zero to lzero ; suc to lsucc)

open import Relation.Binary.PropositionalEquality using (_â‰¡_ ; refl ; trans ; cong ; sym)

open import Categories.Category.Core

module Core.Core where

open Category

X : Category lzero lzero lzero
Obj X = (â„• Ã— â„•) + ğŸ™
(X â‡’ inl x) (inl y) = x â‰¡ y
(X â‡’ inl (k , l)) (inr y) = Fin (k +â„• l)
(X â‡’ inr x) (inl y) = âŠ¥
(X â‡’ inr x) (inr y) = ğŸ™
_â‰ˆ_ X {inl x} {inl .x} refl refl = x â‰¡ x
_â‰ˆ_ X {inl x} {inr y} a b = a â‰¡ b
_â‰ˆ_ X {inr x} {inr y} âˆ— âˆ— = ğŸ™
id X {inl x} = refl
id X {inr âˆ—} = âˆ—
_âˆ˜_ X {inl a} {inl b} {inl c} g f = trans f g
_âˆ˜_ X {inl a} {inl .a} {inr c} g refl = g
_âˆ˜_ X {inl a} {inr b} {inr c} g f = f
_âˆ˜_ X {inr a} {inr b} {inr c} g f = âˆ—
assoc X {inl a} {inl .a} {inl .a} {inl .a} {refl} {refl} {refl} = refl
assoc X {inl a} {inl .a} {inl .a} {inr âˆ—} {refl} {refl} {h} = {!  !}
assoc X {inl a} {inl .a} {inr c} {inr d} {refl} {g} {âˆ—} = {!  !}
assoc X {inl (fstâ‚ , sndâ‚)} {inr âˆ—} {inr âˆ—} {inr âˆ—} {f} {âˆ—} {âˆ—} = {!   !}
assoc X {inr a} {inr b} {inr c} {inr d} {âˆ—} {âˆ—} {âˆ—} = âˆ—
sym-assoc X = {!   !}
identityË¡ X = {!   !}
identityÊ³ X = {!   !}
identityÂ² X = {!   !}
equiv X = {!   !}
âˆ˜-resp-â‰ˆ X = {!   !}  

-- _âˆ˜_ X {inl a} {inl b} {inl c} g f = trans f g
-- _âˆ˜_ X {inl a} {inl b} {inr c} g f = p6 where 
--     p1 : âˆ€ {a b c d} â†’ a â‰¡ c â†’ b â‰¡ d â†’ a +â„• b â‰¡ c +â„• d
--     p1 refl refl = refl
--     p2 : (a b : â„• Ã— â„•) â†’ a â‰¡ b â†’ fst a â‰¡ fst b
--     p2 a b refl = refl
--     p3 : (a b : â„• Ã— â„•) â†’ a â‰¡ b â†’ snd a â‰¡ snd b
--     p3 a b refl = refl
--     p4 : b â‰¡ a
--     p4 = sym f
--     p5 : fst b +â„• snd b â‰¡ fst a +â„• snd a
--     p5 = p1 (p2 b a p4) (p3 b a p4)
--     p6 : Fin (fst a +â„• snd a)
--     p6 = fin-same g p5 